

A Circular Lemma

2002. *Proposed by Dorin Marghidanu, Colegiul National "A. I. Cuza," Corabia, Romania.*

Let a_1, a_2, \dots, a_n be positive real numbers. Prove that

$$\frac{a_1^2}{a_1 + a_2} + \frac{a_2^2}{a_2 + a_3} + \dots + \frac{a_{n-1}^2}{a_{n-1} + a_n} + \frac{a_n^2}{a_n + a_1} \geq \frac{a_1 + a_2 + \dots + a_n}{2}.$$

Solution by Winona State Problem Solvers, Winona State University, Winona, MN.

We require two lemmas to prove the main result. The first is a basic technical result.

Lemma 1: For any nonnegative real numbers a_i and a_j ,

$$\frac{a_i^2}{a_i + a_j} + \frac{a_j^2}{a_j + a_i} \geq \frac{a_i + a_j}{2}.$$

Proof: Consider

$$\begin{aligned} (a_i - a_j)^2 &\geq 0 \\ 2a_i^2 + 2a_j^2 &\geq a_i^2 + a_j^2 + 2a_i a_j \\ 2(a_i^2 + a_j^2) &\geq (a_i + a_j)^2 \\ \frac{a_i^2 + a_j^2}{a_i + a_j} &\geq \frac{a_i + a_j}{2}. \end{aligned}$$

The next lemma is a curious identity that will allow us to shift our numerators.

Lemma 2: For any finite collection of nonnegative real numbers a_i ,

$$\frac{a_1^2}{a_1 + a_2} + \frac{a_2^2}{a_2 + a_3} + \dots + \frac{a_{n-1}^2}{a_{n-1} + a_n} + \frac{a_n^2}{a_n + a_1} = \frac{a_2^2}{a_1 + a_2} + \frac{a_3^2}{a_2 + a_3} + \dots + \frac{a_n^2}{a_{n-1} + a_n} + \frac{a_1^2}{a_n + a_1}.$$

Proof: We proceed by induction. The base case ($n = 2$) is trivial. Assume the inductive hypothesis for k :

$$\sum_{i=1}^{k-1} \frac{a_i^2}{a_i + a_{i+1}} + \frac{a_k^2}{a_k + a_1} = \sum_{i=2}^k \frac{a_i^2}{a_{i-1} + a_i} + \frac{a_1^2}{a_k + a_1}. \quad (1)$$

Then for the $k + 1$ case, we have the expression

$$\sum_{i=1}^{k-1} \frac{a_i^2}{a_i + a_{i+1}} + \frac{a_k^2}{a_k + a_{k+1}} + \frac{a_{k+1}^2}{a_{k+1} + a_1}. \quad (2)$$

Solving for the summation in (1) and substituting into (2) yields

$$\begin{aligned}
 (2) &= \sum_{i=2}^k \frac{a_i^2}{a_{i-1} + a_i} + \frac{a_1^2}{a_k + a_1} - \frac{a_k^2}{a_k + a_1} + \frac{a_k^2}{a_k + a_{k+1}} + \frac{a_{k+1}^2}{a_{k+1} + a_1} \\
 &= \sum_{i=2}^k \frac{a_i^2}{a_{i-1} + a_i} - \frac{(a_k + a_1)(a_k - a_1)}{a_k + a_1} + \frac{a_k^2}{a_k + a_{k+1}} + \frac{a_{k+1}^2}{a_{k+1} + a_1} \\
 &= \sum_{i=2}^k \frac{a_i^2}{a_{i-1} + a_i} - \frac{a_k(a_k + a_{k+1})}{a_k + a_{k+1}} + \frac{a_k^2}{a_k + a_{k+1}} + \frac{a_1(a_{k+1} + a_1)}{a_{k+1} + a_1} + \frac{a_{k+1}^2}{a_{k+1} + a_1} \\
 &= \sum_{i=2}^k \frac{a_i^2}{a_{i-1} + a_i} - \frac{a_k a_{k+1}}{a_k + a_{k+1}} + \frac{a_1 a_{k+1}}{a_{k+1} + a_1} + \frac{a_1^2}{a_{k+1} + a_1} + \frac{a_{k+1}^2}{a_{k+1} + a_1} \\
 &= \sum_{i=2}^k \frac{a_i^2}{a_{i-1} + a_i} + \frac{(a_1 a_{k+1} + a_{k+1}^2)(a_k + a_{k+1}) - a_k a_{k+1}(a_{k+1} + a_1)}{(a_{k+1} + a_1)(a_k + a_{k+1})} + \frac{a_1^2}{a_{k+1} + a_1} \\
 &= \sum_{i=2}^k \frac{a_i^2}{a_{i-1} + a_i} + \frac{a_{k+1}^2(a_{k+1} + a_1)}{(a_{k+1} + a_1)(a_k + a_{k+1})} + \frac{a_1^2}{a_{k+1} + a_1} \\
 &= \sum_{i=2}^k \frac{a_i^2}{a_{i-1} + a_i} + \frac{a_{k+1}^2}{(a_k + a_{k+1})} + \frac{a_1^2}{a_{k+1} + a_1}.
 \end{aligned}$$

Main Proposition For any finite collection of real numbers a_i ,

$$\sum_{i=1}^{n-1} \frac{a_i^2}{a_i + a_{i+1}} + \frac{a_n^2}{a_n + a_1} \geq \sum_{i=1}^n \frac{a_i}{2}.$$

Proof: Consider the left hand side of the desired inequality

$$\begin{aligned}
 \text{LHS} &= \sum_{i=1}^{n-1} \frac{a_i^2}{a_i + a_{i+1}} + \frac{a_n^2}{a_n + a_1} \\
 &= \left(\sum_{i=1}^{n-1} \frac{a_i^2}{a_i + a_{i+1}} + \frac{a_{i+1}^2}{a_{i+1} + a_i} \right) - \sum_{i=1}^{n-1} \frac{a_{i+1}^2}{a_{i+1} + a_i} + \left(\frac{a_n^2}{a_n + a_1} + \frac{a_1^2}{a_n + a_1} \right) - \frac{a_1^2}{a_n + a_1} \\
 &\geq \sum_{i=1}^{n-1} \frac{a_i + a_{i+1}}{2} + \frac{a_n + a_1}{2} - \left(\sum_{i=1}^{n-1} \frac{a_{i+1}^2}{a_{i+1} + a_i} + \frac{a_1^2}{a_n + a_1} \right) \quad (\text{by Lemma 1}) \\
 &= \sum_{i=1}^n a_i - \text{LHS} \quad (\text{by Lemma 2}).
 \end{aligned}$$

Now adding the LHS to both sides and dividing by 2 yields the desired result.